some work on fixtyping

src/FcEtt/fix_typing.v
@@ -161,60 +161,90 @@ Proof.
   eauto. 
 Qed.
 
-Definition FixPat : tm := a_App (a_App (a_Fam Fix) (Rho Irrel) a_Bullet) (Rho Rel) (a_Var_f FixVar2).
+Definition FixPat : tm := 
+    a_App (a_App (a_Fam Fix) (Rho Irrel) a_Bullet) (Rho Rel) (a_Var_f FixVar2).
 
 Definition FixCtx : context := 
   ( FixVar2 , Tm (a_Pi Rel (a_Var_f FixVar1) (a_Var_f FixVar1))) :: ( FixVar1 , Tm a_Star) :: nil.
 
+Definition BodyTy : tm := (a_Var_f FixVar1).
+
+Lemma diff_vars : FixVar1 <> FixVar2.
+Proof. 
+  unfold FixVar1, FixVar2.
+  destruct constants as [s [f [f1 [f2 [j k]]]]].
+  split_hyp.
+  fsetdec.
+Qed.
+
 Lemma CtxFixCtx : Ctx FixCtx.
 Proof.
   unfold FixCtx. 
-  have h: Ctx [( FixVar1 , Tm a_Star)]. econstructor; eauto 2.
+  have h: Ctx [( FixVar1 , Tm a_Star)].
   econstructor; eauto 2.
-  + pick fresh x excluding {{ FixVar1 }} and apply E_Pi.
-    eapply E_Pi with (L := {{ FixVar1 }}).
-    simpl.
-
-Lemma FixDef_FixTy_erase :
-  Typing nil (erase_tm FixDef Nom) (erase_tm FixTy Nom).
-Proof.
-  pose (H := AxFix). clearbody H.
-  unfold FixDef,FixTy; simpl.
-  use_binder E_Abs X.
-  use_binder E_Abs x.
-  { use_binder E_Pi Z. eauto. }
-  { eapply E_App_intro; eauto.
-    { eapply E_App_intro; simpl; eauto.
-      { eapply E_IApp_intro with (a := (a_Var_f X)); simpl; eauto.
-        pose (K := @E_Fam _ Fix (erase_tm FixTy Nom) Nom (erase_tm FixDef Nom) Nom Nom H1).
-        unfold toplevel, erase_sig in K.
-        apply binds_map with 
-          (f:=fun s : sig_sort => erase_csort s Nom) in H.
-        apply K in H.
-        clear K.
-        simpl in H.
-        rewrite param_same.
-        apply H.
-
-        { simpl.
-        use_binder E_Pi Z; eauto.
-        use_binder E_Pi W; eauto.
-        use_binder E_Pi M; eauto.
-        use_binder E_Pi N; eauto. }
-
-        { unfold open_tm_wrt_tm. simpl. eauto. }
-      }
-      unfold open_tm_wrt_tm. simpl. eauto.
-    }
-  }
-  use_binder E_Pi Z; eauto. Unshelve. all: exact Rep.
+  econstructor; eauto 2.
+  use_binderL E_Pi X {{ FixVar1 }}.
+  eauto.
+  simpl.
+  pose k:= diff_vars. clearbody k. fsetdec.
 Qed.
-*)
 
-Lemma Sig_toplevel: Sig toplevel. Proof. Admitted.
-(*Proof.
-  unfold toplevel, erase_sig.
-  unfold an_toplevel.
-  econstructor; eauto.
-  eapply FixDef_FixTy_erase.
-Qed. *)
+Lemma FixDef_FixTy :
+  Typing FixCtx FixDef BodyTy.
+Proof.
+  unfold FixCtx,FixDef,BodyTy; simpl.
+  { eapply E_App_intro; eauto 1.
+    + econstructor; eauto using CtxFixCtx.
+    + cbn. auto.
+    + eapply E_App_intro; simpl; eauto.
+      { eapply E_IApp_intro with (a := (a_Var_f FixVar1)); simpl; eauto.
+        eapply E_Fam; eauto using CtxFixCtx.
+        unfold toplevel, ett_ott.FixTy.
+        eauto.
+        eapply FixTy_typing; eauto.
+        cbn. eauto.
+        eapply E_Var; eauto using CtxFixCtx.
+      } 
+      cbn. auto.
+      eapply E_Var; eauto using CtxFixCtx.
+  } 
+Qed.
+
+Definition FixRolCtx := ( FixVar2 , Nom ) :: nil.
+
+
+Lemma Fix_roleing : roleing FixRolCtx FixDef Nom.
+Proof. 
+  unfold FixRolCtx, FixDef.
+  econstructor; eauto 2.
+  econstructor; eauto 2.
+  econstructor; eauto 2.
+  econstructor; eauto 2.
+  eapply role_a_Fam; eauto 2.
+  unfold toplevel; eauto.
+  eauto.
+  eauto.
+Qed. 
+
+Lemma FixPatCtx : PatternContexts FixRolCtx FixCtx [ FixVar1 ] Fix FixTy FixPat BodyTy.
+Proof.
+  unfold FixRolCtx, FixCtx, FixPat, FixTy, BodyTy.
+  simpl_env.
+Admitted.
+
+Definition toplevel : sig := Fix ~ Ax FixPat FixDef FixTy Nom [Nom].
+
+Lemma Sig_toplevel: Sig toplevel. Proof. 
+  unfold toplevel.
+  simpl_env.
+  replace [Nom] with (range FixRolCtx).
+  eapply Sig_ConsAx; eauto 2.
+  eapply FixTy_typing.
+  eapply FixPatCtx.
+  eapply FixDef_FixTy.
+  move=> x In. simpl in *. destruct In. subst. 
+  pose k:= diff_vars. move => h. apply k. fsetdec.
+  done.
+  eapply Fix_roleing.
+  cbn. auto.
+Qed.
